meta-same mostly done, start of meta-inst

template-coq/theories/Unification.v
@@ -7,6 +7,7 @@ From Coq.FSets Require Import FMapAVL.
 From MetaCoq.Utils Require Import utils.
 From MetaCoq.Common Require Import BasicAst uGraph config.
 From MetaCoq.Template Require Import Ast AstUtils Checker.
+Import MCMonadNotation.
 
 Unset Guard Checking.
 
@@ -14,74 +15,154 @@ Unset Guard Checking.
 Notation "f $ x" := (f x) 
   (at level 10, x at level 100, right associativity, only parsing).
 
+(** Right-to-left function composition. *)
+Notation "f <<< g" := (fun x => f (g x)) (at level 40, left associativity).
+
+(** Left-to-right function composition. *)
+Notation "f >>> g" := (fun x => g (f x)) (at level 40, left associativity).
+
+(** Unification flags. *)
+(** TODO : document them. *)
+Record unif_flags :=
+  { uf_beta_reduce_type : bool
+  ; uf_unify_types : bool 
+  ; uf_aggressive : bool
+  ; uf_super_aggressive : bool 
+  ; uf_try_solving_eqn : bool }.
+
 (** * Evar map. *)
+
+(** Evar identifiers. *)
+Definition evar := nat.
 
 (** An evar entry in the evar map. *)
 Record evar_entry := 
-  { ev_name : aname 
-  ; ev_type : term 
-  ; ev_def  : option term }.
+  { (** The evar's name. For printing only. *)
+    ev_name : name 
+  ; (** The evars' named context. The declarations in this context
+        should contain no loose de Bruijn index (tRels). *)
+    ev_nctx : named_context
+  ; (** The evar's conclusion. It should be well-typed in the evar's context. *)
+    ev_concl : term 
+  ; (** If evar's definition (or None if the evar is undefined).
+        It should be well-typed in the evar's context. *)
+    ev_def : option term }.
+
+(** Maps indexed by evars. *)
+Module EvarOT := OrderedTypeEx.Nat_as_OT.
+Module EMap := FMapAVL.Make EvarOT.
 
 Module EvarMap.
 
-(** [NatMap T] are maps from natural numbers to elements of type [T]. *)
-(** TODO : use binary numbers (or even primitive integers) instead of nats for the keys. *)
-Module NatMap := FMapAVL.Make (OrderedTypeEx.Nat_as_OT).
-
-(** An evar map is a map from evar identifiers to entries. *)
-Definition t := NatMap.t evar_entry.
+(** The type of evar maps. *)
+Record t := 
+  { (** A map from evars to evar entries. *)
+    evm_map : EMap.t evar_entry
+  ; (** A counter used to generate fresh evars. *)
+    evm_counter : nat }.
 
 (** The empty evar map. *)
-Definition empty : t := @NatMap.empty evar_entry.
+Definition empty : t := {| evm_map := @EMap.empty evar_entry ; evm_counter := 0 |}.
 
-(** [evar_type evm ev] retrieves the type of evar [ev] in the evar map [evm]. *)
-Definition evar_type evm ev : option term :=
-  match NatMap.find ev evm with 
-  | None => None 
-  | Some entry => Some entry.(ev_type)
-  end. 
+(** Lookup the entry of an evar in the evar map. *)
+Definition lookup (evm : t) (ev : evar) : option evar_entry :=
+  EMap.find ev evm.(evm_map).
+
+(** [evar_concl evm ev] retrieves the conclusion of evar [ev] in the evar map [evm]. *)
+Definition evar_concl (evm : t) (ev : evar) : option term := 
+  option_map ev_concl $ lookup evm ev.
 
 (** [evar_def evm ev] retrieves the definition of evar [ev] in the evar map [evm]. *)
-Definition evar_def evm ev : option term :=
-  match NatMap.find ev evm with 
+Definition evar_def (evm : t) (ev : evar) : option term :=
+  match EMap.find ev evm.(evm_map) with 
   | None => None 
   | Some entry => entry.(ev_def)
   end.
   
-Definition add evm ev entry : EvarMap.t :=
-  NatMap.add ev entry evm.
+(** [is_defined evm ev] checks if [ev] is present in [evm] and is defined. *)
+Definition is_defined (evm : t) (ev : evar) : bool :=
+  match evar_def evm ev with 
+  | Some _ => true 
+  | None => false 
+  end.
 
-(* Precondition : [ev] is present in [evm] but not defined. *)
-Definition define evm ev def : EvarMap.t :=
-  match NatMap.find ev evm with 
+(** [define evm ev def] assignes [ev := def] in the evar map [evm].
+    This assumes : 
+    - [ev] is present in [evm] but not defined.
+    - [def] is well-type in the context of [ev]. *)
+Definition define (evm : t) (ev : evar) (def : term) : t :=
+  match EMap.find ev evm.(evm_map) with 
   | None => evm 
   | Some e => 
     let e : evar_entry := 
-      {| ev_name := e.(ev_name) 
-      ;  ev_type := e.(ev_type)
+      {| ev_name := e.(ev_name)
+      ;  ev_nctx := e.(ev_nctx) 
+      ;  ev_concl := e.(ev_concl)
       ;  ev_def  := Some def |}
     in
-    NatMap.add ev e evm
+    {| evm_map := EMap.add ev e evm.(evm_map) ; evm_counter := evm.(evm_counter) |}
   end.
 
+Definition new_evar (evm : t) (nctx : named_context) (concl : term) : (t * evar) :=
+  let entry := 
+    {| ev_name := nNamed "x"%bs 
+    ;  ev_nctx := nctx 
+    ;  ev_concl := concl 
+    ;  ev_def := None |}
+  in 
+  let ev := evm.(evm_counter) in
+  (* Don't forget to increment the evar counter. *)
+  let evm := 
+    {| evm_map := EMap.add ev entry evm.(evm_map) ; evm_counter := S evm.(evm_counter) |}
+  in
+  (evm, ev).
+  
 End EvarMap.
+
+
+(** [subst_var v t u] replaces all occurences of [v] by [t] in [u].
+    It assumes [t] contains no loose tRel (i.e. it does not perform lifting). *)
+Fixpoint subst_var (v : ident) (t u : term) : term :=
+  match u with 
+  | tVar v' => if v == v' then t else tVar v'
+  | _ => map_term (subst_var v t) u
+  end.
+
+(** [instantiate_evar ctx subs def] instantiates an evar. 
+    - [ctx] is the named context of the evar. 
+    - [def] is the definition of the evar.
+    - [subs] is the list of terms which are substituted for the variables in [ctx].
+    TODO : make this more efficient. *)
+Fixpoint instantiate_evar (ctx : named_context) (subs : list term) (def : term) : term :=
+  match ctx, subs with 
+  | (id, _) :: ctx, s :: subs =>
+    instantiate_evar ctx subs (subst_var id s def)
+  | _, _ => def 
+  end.
 
 (** [nf_evars evm t] replaces all defined evars that appear in [t] 
     by their body. *)
-Definition nf_evars (evm : EvarMap.t) (t : term) : term. 
-(* TODO : use map_term. *)
-Admitted.
+Fixpoint nf_evars (evm : EvarMap.t) (t : term) {struct t} : term :=
+  match t with 
+  | tEvar ev subs =>
+    match EvarMap.lookup evm ev with 
+    | Some {| ev_name := _ ; ev_nctx := ctx ; ev_concl := _ ; ev_def := Some def |} =>
+      nf_evars evm $ instantiate_evar ctx subs def 
+    | _ => t 
+    end 
+  | _ => map_term (nf_evars evm) t
+  end.
 
 (** [whd_evars evm t] expands evars just enough to expose the first 
     constructor which is not [tEvar] in [t]. *)
 Fixpoint whd_evars (evm : EvarMap.t) (t : term) {struct t} : term :=
   match t with 
-  | tEvar ev [] => 
-    match EvarMap.evar_def evm ev with 
-    | None => t 
-    | Some def => whd_evars evm def
-    end
-  (* TODO : evars with an instance. *)
+  | tEvar ev subs =>
+    match EvarMap.lookup evm ev with 
+    | Some {| ev_name := _ ; ev_nctx := ctx ; ev_concl := _ ; ev_def := Some def |} =>
+      whd_evars evm $ instantiate_evar ctx subs def 
+    | _ => t 
+    end 
   | _ => t 
   end.
 
@@ -125,16 +206,13 @@ Definition concat (l l' : t) : t := List.app l l'.
 
 End Log.*)
 
-(** Monadic return. *)
-Definition ret {A} (a : A) : unif_result A := Success a.
-
 (** Monadic bind. *)
-Definition bind {A} {B} (ma : unif_result A) (mf : A -> unif_result B) : unif_result B :=
+Definition bind_ {A} {B} (ma : unif_result A) (mf : A -> unif_result B) : unif_result B :=
   match ma with 
   | Success a => mf a 
   | UnifError err => UnifError err
   end.
-Notation "'let*' x := c1 'in' c2" := (bind c1 (fun x => c2))
+Notation "'let*' x := c1 'in' c2" := (bind_ c1 (fun x => c2))
   (at level 100, x pattern, c1 at next level, right associativity).
 
 (** Monadic alternative. *)
@@ -149,7 +227,7 @@ Notation "x <|> y" := (msum x y) (at level 85, right associativity).
     [None] is mapped to [UnifError (InternalError ...)]. *)
 Definition lift_option {A} (x : option A) : unif_result A :=
   match x with 
-  | Some x => ret x
+  | Some x => Success x
   | None => UnifError (InternalError "lift_option")
   end.
 
@@ -159,6 +237,7 @@ Definition lift_option {A} (x : option A) : unif_result A :=
 
 (** * Unification algorithm. *)
 
+(** [is_evar evm t] checks if [t] is an evar. *)
 Definition is_evar evm t : bool :=
   match whd_evars evm t with 
   | tEvar _ _ => true 
@@ -168,7 +247,7 @@ Definition is_evar evm t : bool :=
 Fixpoint ise_list2 {A B} (f : A -> B -> EvarMap.t -> unif_result EvarMap.t) 
   (xs : list A) (ys : list B) (evm : EvarMap.t) : unif_result EvarMap.t :=
   match xs, ys with 
-  | [], [] => ret evm 
+  | [], [] => Success evm 
   | x :: xs, y :: ys =>
     let* evm := f x y evm in ise_list2 f xs ys evm
   | _, _ => UnifError NotSameHead
@@ -197,10 +276,235 @@ Definition rebuild_case Σ ci pred bs : option (term * list term) :=
     Some (pred_term, bs_terms)
   end.
 
+(** [find_unique cond xs] checks if there is exactly one element in [xs] that satisfies
+    the condition [cond], and if so returns its index. *)
+Definition find_unique {A} (cond : A -> bool) (xs : list A) : option nat :=
+  (* Loop over elements of [xs] from first to last. 
+     - [i] is the index of the current element.
+     - [res] is [None] if we have not yet found an element satisfying [cond],
+       otherwise it is [Some idx] where [idx] is the position of the element. *)
+  let fix loop res i xs :=
+    match xs with 
+    | [] => res 
+    | x :: xs =>
+      if cond x then 
+        match res with 
+        (* We found a first element satisfying [cond]. *)
+        | None => loop (Some i) (S i) xs 
+        (* We found two elements satisfying [cond] : return [None]. *)
+        | Some _ => None 
+        end
+      else loop res (S i) xs
+    end 
+  in 
+  loop None 0 xs.
+  
+(** Specialization of [find_unique] to named variables (tVars). *)
+Definition find_unique_var evm (id : ident) (ts : list term) :=
+  find_unique (fun t => whd_evars evm t == tVar id) ts.
+
+(** Specialization of [find_unique] to de Bruijn variables (tRels). *)
+Definition find_unique_rel evm (n : nat) (ts : list term) :=
+  find_unique (fun t => whd_evars evm t == tRel n) ts.
+
+Module Invert.
+
+(** We need a state-option monad in this section. *)
+Local Definition M A := EMap.t (list nat) -> option (EMap.t (list nat) * A).
+
+#[local] Instance : Monad M :=
+{ 
+  ret _ a s := Some (s, a) ;
+  bind _ _ ma mf s := 
+    match ma s with 
+    | None => None
+    | Some (s, a) => mf a s
+    end
+}.
+
+(** Monadic alternative. *)
+Definition msum {A} (mx my : M A) : M A :=
+  fun s =>
+  match mx s with 
+  | None => my s 
+  | Some (s, x) => Some (s, x)
+  end.
+#[local] Notation "x <|> y" := (msum x y) 
+  (at level 85, right associativity).
+   
+Local Definition fail {A} : M A := fun s => None.
+
+Definition invert (evm : EvarMap.t) (map : EMap.t (list nat)) (nctx : named_context) 
+  (ev0 : evar) (subs : list term) (args : list term) (t : term) : option (EMap.t (list nat) * term) :=
+  let subs_args := subs ++ args in
+  let var_or_rel depth k :=
+    if k <? #|subs| 
+    then option_map (tVar <<< fst) $ List.nth_error nctx k
+    else Some $ tRel $ #|subs_args| - k - 1 + depth
+  in 
+  let fix invert_aux (inside_evar : bool) (depth : nat) (t : term) : M term :=
+    match whd_evars evm t with
+    | tVar id =>
+      match var_or_rel depth =<< find_unique_var evm id subs_args with
+      | None => fail 
+      | Some t => ret t
+      end
+    | tRel j =>
+      if depth <? j then 
+        match var_or_rel depth =<< find_unique_rel evm (j - depth) subs_args with 
+        | None => fail 
+        | Some t => ret t
+        end
+      else ret $ tRel j
+    | tEvar ev args =>
+      if ev == ev0 then fail else 
+	  (*let evargs' := Evd.expand_existential sigma (ev', evargs') in*)
+	  let on_arg arg_idx arg := 
+        (* First try to invert the argument. *)
+        invert_aux true depth arg <|>
+        (* We could not invert this argument : we have to prune it. *)
+		(* Pruning can not happen inside an evar's suspended substitution. *)
+        if inside_evar then fail else 
+        (* Extend the pruning map : we have to prune the declaration 
+           at position [arg_idx] of evar [ev]. *)
+        (fun map => 
+		  let prev_idxs := option_get [] (EMap.find ev map) in
+          let map := EMap.add ev (arg_idx :: prev_idxs) map in 
+          Some (map, arg))
+	  in
+      (* Invert each argument. *)
+      mlet args <- monad_map_i on_arg args ;;
+      ret $ tEvar ev args
+	| _ =>
+      map_term_with_bindersM depth (fun _ depth => ret $ S depth) (invert_aux inside_evar) t
+    end
+  in
+  invert_aux false 0 t map.
+
+End Invert.
+
+(** [invert evm map nctx ev subs args t] inverts the equation [?ev[subst] args := t]
+    (where [nctx] is the named context of the evar, thus #|nctx| = #|subs|).
+    
+    More precisely it builds a term t' equal to t, except that every free variable 
+    (tVar or tRel) x in t is replaced by :
+    - if x appears does not appear _uniquely_ in [subs ++ args], then we fail.
+    - if x appears in [subs] at index [i], then x is replaced by [tVar n]
+      where [n] is the name of the variable in [nctx] at index [i].
+    - If x appears in [args] at index [i] (starting from the end), 
+      then x is replaced by [tRel i].
+    It fails if [ev] appears inside [t]. 
+    
+    This function implements a heuristic which helps in some cases : it tries to 
+    prune evars appearing in [t] (see also the [prune] function). 
+    [map] is the initial pruning map (which assign to every evar a list of argument
+    positions to prune), which [invert] extends as needed. *)
+Definition invert := Invert.invert.
+
+(** [term_fvars evm t] computes the set of free variables (tVars) in the term [t]. *)
+Definition term_fvars (evm : EvarMap.t) (t : term) : IdentSet.t := 
+  let fix aux acc t :=
+    match whd_evars evm t with 
+    | tVar v => IdentSet.add v acc 
+    | _ => fold_term_with_binders tt (fun _ _ => tt) (fun _ => aux) acc t 
+    end 
+  in 
+  aux IdentSet.empty t.
+
+(** [has_free_var evm vars t] checks if [t] has a free variable which is in [vars]. *)
+Definition has_free_var (evm : EvarMap.t) (vars : list ident) (t : term) : bool :=
+  let fvars := term_fvars evm t in 
+  List.existsb (fun v => IdentSet.mem v fvars) vars.
+
+(** [remove_with_deps evm nctx pos] removes the declarations at positions [pos] in named context [nctx].
+    Declarations which depend on removed ones are removed as well. *)
+Definition remove_with_deps (evm : EvarMap.t) (nctx : named_context) (pos : list nat) : named_context :=
+  (* We process declarations in [nctx] from last to first (i.e. outermost to innermost).
+     - [i] is the index of the current declaration.
+     - [removed] contains the identifiers of the variables which were removed so far. *)
+  let fix loop i nctx removed :=
+    match nctx with
+    | [] => []
+    | (id, d) :: nctx =>
+      if List.existsb (eqb i) pos
+         || has_free_var evm removed d.(decl_type) 
+         || option_default (has_free_var evm removed) d.(decl_body) false
+      (* Remove [d]. *)
+      then loop (pred i) nctx (id :: removed)
+      (* Keep [d]. *)
+      else (id, d) :: loop (pred i) nctx removed
+    end
+  in
+  rev $ loop (pred #|nctx|) (rev nctx) [].
+      
+(** [prune evm ev pos] prunes the declarations at positions [pos] in the context of the evar [ev].
+    More precisely :
+    - if [ev] is defined in [evm] it does nothing.
+    - if [ev] is undefined in [evm], it assigns [ev := ev'] where [ev'] has the same conclusion
+      as [ev] but lives in a context which has been pruned. 
+    It returns [None] if prunning failed. *)
+Fixpoint prune (evm : EvarMap.t) (ev : nat) (pos : list nat) {struct ev} : option EvarMap.t :=
+  if EvarMap.is_defined evm ev then Some evm else
+  mlet entry <- EvarMap.lookup evm ev ;; 
+  (* Remove the required positions from the local context of the evar. *)
+  let new_ctx := remove_with_deps evm entry.(ev_nctx) pos in 
+  (* Make sure the conclusion of the evar does not contain any removed variables.
+     This might require pruning other evars which appear in the conclusion. *)
+  let concl := entry.(ev_concl) in
+  let new_ctx_vars := List.map (tVar <<< fst) new_ctx in
+  mlet '(map, _) <- invert evm (EMap.empty (list nat)) new_ctx ev new_ctx_vars [] concl ;;
+  (* Prune other evars as needed. *)
+  mlet evm <- prune_all evm map tt ;;
+  (* Create a fresh evar [ev'] in the new context. *)
+  let (evm, ev') := EvarMap.new_evar evm new_ctx concl in
+  (* Assign [ev := ev']. *)
+  Some $ EvarMap.define evm ev' (tEvar ev new_ctx_vars)
+
+(** [prune_all evm map tt] prunes all the evars in [evm] according to [map].
+    Unfortunately for technical reasons we have to pass a useless [tt] argument to [prune_all]. *)
+with prune_all (evm : EvarMap.t) (map : EMap.t (list nat)) (dummy : unit) {struct dummy} : option EvarMap.t :=
+  monad_fold_left (fun evm '(ev, pos) => prune evm ev pos) (EMap.elements map) evm. 
+
 Section Algorithm.
-Context `{cf : checker_flags} (φ : universes_graph) (Σ : global_env) (Δ : named_context).
+Context `{uf : unif_flags} `{cf : checker_flags} (φ : universes_graph) (Σ : global_env) (Δ : named_context).
 
 Implicit Types (pb : conv_pb) (Γ : context).
+
+(** [intersect evm xs ys] computes the list of positions where the terms in [xs] and [ys] 
+    are not equal. By default only disagreements on positions where both are variables 
+    (tVar or tRel) are accepted, and we return None otherwse.
+    The unification flag [uf_aggressive] bypasses this behaviour, making [intersect] always succeed. *)
+Definition intersect evm (xs ys : list term) : option (list nat) :=
+  let is_var t := 
+    match whd_evars evm t with tVar _ | tRel _ => true | _ => false end 
+  in  
+  let fix loop i xs ys diff :=
+    match xs, ys with 
+    | [], [] => Some diff
+    | x :: xs, y :: ys =>
+      if eq_term φ x y then loop (S i) xs ys diff 
+      else if is_var x && is_var y then loop (S i) xs ys (i :: diff)
+      else if uf.(uf_aggressive) then loop (S i) xs ys (i :: diff)
+      else None
+    | _, _ => None 
+    end 
+  in 
+  loop 0 xs ys [].
+          
+(** [meta_same evm ev subs1 subs2] implements the Meta-Same rule to unify [ev[subs1] =?= ev[subs2]]. *)
+Definition meta_same evm (ev : evar) (subs1 subs2 : list term) : unif_result EvarMap.t :=
+  (* Prune the evar on the positions where [subs1] and [subs2] disagree. *)
+  match intersect evm subs1 subs2 with
+  | Some [] => 
+    (* Fast path to avoid pruning if unnecessary. *) 
+    Success evm
+  | Some pos =>
+    match prune evm ev pos with 
+    | Some evm => Success evm 
+    | None => UnifError NotSameHead
+    end
+  | None => UnifError NotSameHead
+  end.
 
 (** Main unification function. *)
 Fixpoint unify pb Γ t t' evm {struct pb} : unif_result EvarMap.t :=
@@ -211,32 +515,49 @@ Fixpoint unify pb Γ t t' evm {struct pb} : unif_result EvarMap.t :=
 (** Precondition : either t or t' is an evar. *)
 with try_instantiate pb Γ t t' evm {struct pb} : unif_result EvarMap.t :=
   match whd_evars evm t, whd_evars evm t' with 
-  | tEvar ev [], tEvar ev' [] => 
+  | tEvar ev subs, tEvar ev' subs' => 
     if ev == ev' 
-    (* Meta-Same : TODO *)
-    then ret evm   
-    (* Try both Meta-InstL and Meta-InstR *)
-    else instantiate pb Γ ev t' evm <|> instantiate pb Γ ev' t evm
+    (* Meta-Same *)
+    then meta_same evm ev subs subs'
+    (* Meta-Meta *)
+    else
+      (* We try both directions, but first the one with the longest substitution. *)
+      let '(ev1, ev2, subs1, subs2, t1, t2) := 
+        if #|subs| <? #|subs'|
+        then (ev', ev, subs', subs, t, t')
+        else (ev, ev', subs, subs', t', t)
+      in 
+      meta_inst pb Γ ev1 subs1 t1 evm <|> 
+      meta_inst pb Γ ev2 subs2 t2 evm
   (* Meta-InstL *)
-  | tEvar ev [], _ => instantiate pb Γ ev t' evm
+  | tEvar ev subs, t0 => meta_inst pb Γ ev subs t0 evm
   (* Meta-InstR *)
-  | _, tEvar ev [] => instantiate pb Γ ev t evm
+  | t0, tEvar ev subs => meta_inst pb Γ ev subs t0 evm
   | _, _ => UnifError (InternalError "try_instantiate : expected an evar")
   end
 
-with instantiate pb Γ ev t evm {struct pb} : unif_result EvarMap.t :=
-  (* Check the evar and t have the same type. *)
+(** [meta_inst pb Γ ev subs t evm] implements the Meta-Inst rule to instantiate [ev[subs] := t]. *)
+with meta_inst pb Γ ev subs t evm {struct pb} : unif_result EvarMap.t :=
+  let is_var t := 
+    match t with tVar _ | tRel _ => true | _ => false end 
+  in
+  (* Check the substitution and arguments contain only variables (tVars and tRels). *)
+  if List.forallb is_var (subs ++ args) then 
+    
+  else UnifError NotSameHead
+
+(* Check the evar and t have the same type. *)
   let* t_ty := 
     match @Checker.infer cf default_fuel Σ φ Δ Γ t with 
-    | Checked t_ty => ret t_ty 
+    | Checked t_ty => Success t_ty 
     | TypeError err => UnifError (InternalError "Attempt to instantiate with an ill-typed term")
     end 
   in 
-  let* ev_ty := lift_option $ EvarMap.evar_type evm ev in
+  let* ev_ty := lift_option $ EvarMap.evar_concl evm ev in
   let* evm := unify pb Γ ev_ty t_ty evm in 
   (* Define the evar. *)
   let evm := EvarMap.define evm ev t in 
-  ret evm
+  Success evm
 
 with try_same_head pb Γ t t' evm {struct pb} : unif_result EvarMap.t :=
   match whd_evars evm t, whd_evars evm t' with 
@@ -249,7 +570,7 @@ with try_same_head pb Γ t t' evm {struct pb} : unif_result EvarMap.t :=
       end
     in 
     (* TODO : add universe constraints if needed. *)
-    if ok then ret evm else UnifError UnivInconsistency
+    if ok then Success evm else UnifError UnivInconsistency
   (* Lam-Same *)
   | tLambda x ty body, tLambda _ ty' body' =>
     let* evm := unify Conv Γ ty ty' evm in 
@@ -264,15 +585,15 @@ with try_same_head pb Γ t t' evm {struct pb} : unif_result EvarMap.t :=
     unify pb (Γ ,, vdef x def ty) body body' evm
   (* Rigid-Same *)
   | tRel n, tRel n' => 
-    if n == n' then ret evm else UnifError NotSameHead
+    if n == n' then Success evm else UnifError NotSameHead
   | tVar v, tVar v' => 
-    if v == v' then ret evm else UnifError NotSameHead
+    if v == v' then Success evm else UnifError NotSameHead
   | tConst c _, tConst c' _ =>
-    if c == c' then ret evm else UnifError NotSameHead
+    if c == c' then Success evm else UnifError NotSameHead
   | tInd ind _, tInd ind' _ =>
-    if ind == ind' then ret evm else UnifError NotSameHead
+    if ind == ind' then Success evm else UnifError NotSameHead
   | tConstruct ind n _, tConstruct ind' n' _ =>
-    if (ind == ind') && (n == n') then ret evm else UnifError NotSameHead  
+    if (ind == ind') && (n == n') then Success evm else UnifError NotSameHead  
   | tProj p t, tProj p' t' =>
     if p == p' then unify Conv Γ t t' evm else UnifError NotSameHead
   | tFix defs n, tFix defs' n'
@@ -300,6 +621,26 @@ with try_same_head pb Γ t t' evm {struct pb} : unif_result EvarMap.t :=
     ise_list2 (unify Conv Γ) ts ts' evm
   | _, _ => UnifError NotSameHead
   end.
+
+End Algorithm.
+
+(****************************)
+(** Testing *)
+
+From MetaCoq.Template Require Import All.
+
+(** Run a template program. *)
+Notation "'$run' f" :=
+  ltac:(
+    let p y := exact y in
+    run_template_program f p
+  ) (at level 0, only parsing).
+
+Definition t1 := $run (tmQuote (fun x => S x + 1)).
+Definition t2 := $run (tmQuote (fun y => S y + 1)).
+
+Definition Σ := fst ($run (tmQuoteRec (fun x => S x + 1))).
+
 
 (** Main unification function entry point. *)
 (*Definition unify_constr (pb : conv_pb) (t1 t2 : term) (s : state) : state := 
